Do not introduce typevars for logical things
This breaks erasure for some constructors because we use the count of
type vars to figure out whether the constructor is extractable.

extraction/examples/ErasureTests.v
@@ -189,11 +189,11 @@ Check eq_refl : ltac:(let x := eval vm_compute in (erase_and_print_type id ex1) 
 
 MetaCoq Quote Recursively Definition ex2 := (forall (A : Type) (P : A -> Prop), @sig A P).
 Check eq_refl : ltac:(let x := eval vm_compute in (erase_and_print_type id ex2) in exact x) =
-                Ok ("A P", "□ → □ → sig A □").
+                Ok ("A", "□ → □ → sig A □").
 
 MetaCoq Quote Recursively Definition ex3 := (forall (A : Type) (P : A -> Prop), { a : A | P a }).
 Check eq_refl : ltac:(let x := eval vm_compute in (erase_and_print_type id ex3) in exact x) =
-                Ok ("A P", "□ → □ → sig A □").
+                Ok ("A", "□ → □ → sig A □").
 
 MetaCoq Quote Recursively Definition ex4 := (forall (A B : Type) (f : A -> B) (n : nat),
                                         Vector.t A n -> Vector.t B n).
@@ -245,7 +245,7 @@ Check eq_refl : ltac:(let x := eval vm_compute in (erase_and_print_type id ex11)
 
 MetaCoq Quote Recursively Definition ex12 := (forall (A : Type) (P : A -> Prop), unit).
 Check eq_refl : ltac:(let x := eval vm_compute in (erase_and_print_type id ex12) in exact x) =
-                Ok ("A P", "□ → □ → unit").
+                Ok ("A", "□ → □ → unit").
 
 MetaCoq Quote Recursively Definition ex13 := (let p := (nat, unit) in fst p × snd p).
 Check eq_refl : ltac:(let x := eval vm_compute in (erase_and_print_type id ex13) in exact x) =
@@ -471,12 +471,10 @@ Inductive IndexedList : Type -> Type :=
 | icons : forall T, T -> IndexedList T -> IndexedList T.
 
 MetaCoq Quote Recursively Definition ex9 := IndexedList.
-Compute erase_and_print_ind_prog ex9.
 Check eq_refl : ltac:(let x := eval vm_compute in (erase_and_print_ind_prog ex9) in exact x) =
                 Err (EraseIndBodyError "IndexedList" (CtorUnmappedTypeVariables "inil")).
 
 MetaCoq Quote Recursively Definition ex10 := Monad.
-Compute erase_and_print_ind_prog ex10.
 Check eq_refl : ltac:(let x := eval vm_compute in (erase_and_print_ind_prog ex10) in exact x) =
                 Err (EraseIndBodyError "Monad" (EraseCtorError "Build_Monad" NotPrenex)).
 
@@ -484,8 +482,6 @@ Inductive ManyParamsInd (A : Type) (P : Prop) (Q : Prop) (B : Type) :=
   MPIConstr : P -> A -> B -> ManyParamsInd A P Q B.
 
 MetaCoq Quote Recursively Definition ex11 := ManyParamsInd.
-
-Compute erase_and_print_ind_prog ex11.
 
 Example ManyParamsInd_test :
   erase_and_print_ind_prog ex11 =
@@ -518,6 +514,17 @@ Example ManyParamsIndNonArity_remove_log_params_test:
   Ok <$ "data ManyParamsIndNonArity A B";
         "| MPINAConstr1 □ □ □ □ □ A B";
         "| MPINAConstr2 □ □ □ □ □ (list □) (prod A B)" $>.
+Proof. vm_compute. reflexivity. Qed.
+
+Inductive PropTypeVarInCtor :=
+  ex13_ctor : Prop -> PropTypeVarInCtor.
+MetaCoq Quote Recursively Definition ex13 := PropTypeVarInCtor.
+Compute erase_and_print_ind_prog ex13.
+
+Example PropTypeVarInCtor_test :
+  erase_and_print_ind_prog ex13 =
+  Ok <$ "data PropTypeVarInCtor";
+        "| ex13_ctor □" $>.
 Proof. vm_compute. reflexivity. Qed.
 
 End erase_ind_tests.
