extraction/theories/Erasure.v
@@ -507,10 +507,8 @@ erase_type Γ erΓ t wat tvars with inspect (reduce_term redβιζ Σ wfΣ Γ t 
 
       | et_view_prod na A B with flag_of_type Γ A _ := {
           (* For logical things, we add a type variable if it's an arity *)
-        | Checked {| is_logical := true ; is_arity := isar |} :=
-          let e := if isar then RelTypeVar (List.length tvars) else RelOther in
-          let tvars' := if isar then tvars ++ [na] else tvars in
-          '(tvars, bt) <- erase_type (Γ,, vass na A) (e :: erΓ)%vector B _ tvars';;
+        | Checked {| is_logical := true |} :=
+          '(tvars, bt) <- erase_type (Γ,, vass na A) (RelOther :: erΓ)%vector B _ tvars;;
           ret (tvars, TArr TBox bt);
 
           (* If the type isn't an arity now, then it's a "normal" type like nat. *)
@@ -883,7 +881,8 @@ Program Definition erase_ind_body
   let the_rest := skipn (P.ind_npars mib) oib_tvars in
   (* we filter out non-arities from the inductive parameters since non-arities
      will not be type variables *)
-  let ind_params_arities_only := filter tvar_is_arity ind_params in
+  let ind_params_arities_only :=
+      filter (fun t => tvar_is_sort t && negb (tvar_is_logical t)) ind_params in
   (* We map type vars in constructors to type vars in the inductive parameters.
      Thus, we only allow the constructor this many type vars *)
   let num_tvars_in_params :=
